compiler/proof_vec/equiv_chacha20.ec
@@ -1,0 +1,174 @@
+require import AllCore IntDiv List Jasmin_model Chacha20_hacl Chacha20_hacl_x2 Chacha20_s_avx2.
+
+(* --------------------------------------------------------------------------- *)
+(* First we prove that the hacl implementation correspond to the hacl_x2       *)
+(* implementation. The last one allows to express most easyly the invariant    *)
+(* for the s-avx version                                                       *)
+
+equiv hacl_x2_quarter_round : 
+  Chacha20_hacl.M.hacl_Impl_Chacha20_quarter_round ~
+  Chacha20_hacl_x2.M.hacl_Impl_Chacha20_quarter_round : ={arg} ==> ={res}.
+proof. by sim. qed.
+
+equiv hacl_x2_rounds_x2 : 
+  Chacha20_hacl.M.hacl_Impl_Chacha20_rounds_x2 ~
+  Chacha20_hacl_x2.M.hacl_Impl_Chacha20_rounds_x2 : 
+    ={k1,k2} ==> ={res}.
+proof.
+  proc=> /=.
+  inline{1} Chacha20_hacl.M.hacl_Impl_Chacha20_rounds.
+  (* One solution is to unroll the loop and then perform some 
+     swap, I prefer to do the proof by induction so that 
+     the proof do not depend of the number of iteration *)
+  swap{1} 4 3. swap{1} 4 -2. swap{1} 5 -1. wp.
+  seq 4 1 : (exists k, 0 <= k /\  
+       10 - i{1} = k /\ i0{1} = i{1} /\ i{2} = i{1} /\ #post).
+  + by auto => />;exists 10.
+  elim * => k;case @[ambient] (0 <= k); last by move=> ?; exfalso => /#.
+  elim /intind: k.
+  + rcondf{1} 1; 1: by auto => /#.
+    rcondf{1} 1; 1: by auto => /#.
+    by rcondf{2} 1;auto => /#.
+  move=> k hk hrec.
+  rcondt{1} 1; 1: by auto => /#.
+  rcondt{2} 1; 1: by auto => /#.
+  rcondt{1} 4.
+  + move=> &2;conseq (_: true) => // /#.
+  swap{1} 4 -2; swap{1} 5 -1.
+  seq 4 2: (10 - i{1} = k /\
+    i0{1} = i{1} /\ i{2} = i{1} /\ st{1} = k1{2} /\ st0{1} = k2{2});last by apply hrec.
+  inline{1} Chacha20_hacl.M.hacl_Impl_Chacha20_double_round.
+  inline{2} Chacha20_hacl_x2.M.hacl_Impl_Chacha20_double_round_x2.
+  swap{1} [6..10] 5.
+  inline{2} Chacha20_hacl_x2.M.hacl_Impl_Chacha20_round_x2.
+  by do !(wp;call hacl_x2_quarter_round);
+    wp;skip => /> &1 h; ring h.
+qed.
+
+equiv hacl_x2_double : 
+  Chacha20_hacl.M.hacl_2rounds ~
+  Chacha20_hacl_x2.M.hacl_2rounds : 
+   ={st1,st2} ==> ={res}.
+proof.
+  proc => /=; sim; call hacl_x2_rounds_x2; sim />.
+qed.
+
+(* --------------------------------------------------------------------------- *)
+
+lemma rol_xor_simplify (w1 w2:W32.t) i si: 
+   w1 = w2 => si = W32.size - i => 0 <= i < W32.size => 
+   (w1 `<<<` i) `^` (w2 `>>>` si) = rol w1 i.
+proof. by move=> 2!-> hi;rewrite rol_xor. qed.
+
+hint simplify rol_xor_simplify.
+
+(* --------------------------------------------------------------------------- *)
+(* hacl-x2 versus s-avx2                                                       *)
+
+lemma x86_VPSHUFD_256_E (w0 w1 w2 w3 w4 w5 w6 w7 :W32.t) m :
+  x86_VPSHUFD_256 (pack8 [w0; w1; w2; w3; w4; w5; w6; w7]) m = 
+  pack2 [x86_VPSHUFD_128 (pack4 [w0; w1; w2; w3]) m;
+         x86_VPSHUFD_128 (pack4 [w4; w5; w6; w7]) m].
+proof. by rewrite /x86_VPSHUFD_256 -pack2_4u32_8u32. qed.
+
+hint simplify (x86_VPSHUFD_256_E, pack2_4u32_8u32).
+
+op rela_i k i (st1 st2:W32.t Array16.t) =
+  pack8 [ 
+          st1.[4*i+(0+k)%%4]; st1.[4*i+(1+k)%%4]; st1.[4*i+(2+k)%%4]; st1.[4*i+(3+k)%%4];
+          st2.[4*i+(0+k)%%4]; st2.[4*i+(1+k)%%4]; st2.[4*i+(2+k)%%4]; st2.[4*i+(3+k)%%4] ].
+
+op rela (st1 st2:W32.t Array16.t) (s:W256.t Array4.t) =
+   s = Array4.init (fun i => rela_i 0 i st1 st2).
+
+(*
+op rela_after (st1 st2:W32.t Array16.t) (s:W256.t Array4.t) = 
+   s = Array4.init (fun i => rela_i i i st1 st2).
+*)
+hint simplify x86_ROL_32_E.
+
+equiv s_avx2_double_round : 
+  Chacha20_hacl_x2.M.hacl_Impl_Chacha20_double_round_x2 ~ 
+  Chacha20_s_avx2.M.chacha20_double_round : 
+    rela st1{1} st2{1} st{2} ==> rela res{1}.`1 res{1}.`2 res{2}.
+proof.
+  proc.
+  seq 1 1: (rela st1{1} st2{1} st{2}).
+  + conseq (: Array4.all_eq st{2}
+                (Array4.init (fun i => rela_i 0 i st1 st2)){1}). 
+    + by move=> ?????? h;apply Array4.ext_eq_all;apply h. 
+    inline *; wp;skip=> &1 &2 h.
+    rewrite $h.
+    by cbv Array4.all_eq rela_i x86_VPADD_8u32 x86_VPSRL_8u32 x86_VPSLL_8u32 (%%) (%/)
+         W32.(`>>`) W32.(`<<`) => /=.
+  conseq (: Array4.all_eq st{2}
+              (Array4.init (fun i => rela_i 0 i st1 st2)){1}). 
+  + by move=> ?????? h;apply Array4.ext_eq_all;apply h. 
+  inline *; wp;skip=> &1 &2 h.
+  rewrite $h.
+  by cbv Array4.all_eq rela_i x86_VPADD_8u32 x86_VPSRL_8u32 x86_VPSLL_8u32 (%%) (%/)
+         W32.(`>>`) W32.(`<<`) x86_VPSHUFD_128 x86_VPSHUFD_128_B => /=.
+qed.
+
+equiv s_avx2_chacha20_rounds :
+  Chacha20_hacl_x2.M.hacl_Impl_Chacha20_rounds_x2 ~
+  Chacha20_s_avx2.M.chacha20_rounds :
+   rela k1{1} k2{1} st{2} ==> rela res{1}.`1 res{1}.`2 res{2}.
+proof.
+  proc.
+  while (={i} /\ rela k1{1} k2{1} st{2});last by auto.
+  by wp; call s_avx2_double_round;skip.
+qed.
+
+equiv s_avx2_copy_states : 
+  Chacha20_hacl_x2.M.hacl_Impl_Chacha20_copy_state_x2 ~ 
+  Chacha20_s_avx2.M.chacha20_copy_state : 
+    rela st1{1} st2{1} s{2} ==> rela res{1}.`1 res{1}.`2 res{2}.
+proof.
+  proc;inline *.
+  unroll for {1} 11;unroll for {1} 6.
+  unroll for {2} 3;wp;skip => />.
+  move=> &1 &2 ->;rewrite /rela;apply Array4.ext_eq_all.
+  by cbv Array4.all_eq rela_i (%%) (%/).
+qed.
+
+equiv s_avx2_sum_states : 
+  Chacha20_hacl_x2.M.hacl_Impl_Chacha20_sum_states_x2 ~ 
+  Chacha20_s_avx2.M.chacha20_sum_states : 
+    rela k1{1} k2{1} k{2} /\
+    rela st1{1} st2{1} s{2} ==> rela res{1}.`1 res{1}.`2 res{2}.
+proof.
+  proc;inline *.
+  unroll for {1} 9;unroll for {1} 4.
+  unroll for {2} 2;wp;skip => &1 &2 /= /> -> ->.
+  apply Array4.ext_eq_all.  
+  by cbv Array4.all_eq rela_i x86_VPADD_8u32 (%%) (%/).
+qed.
+
+equiv s_avx2_2rounds : 
+  Chacha20_hacl_x2.M.hacl_2rounds ~
+  Chacha20_s_avx2.M.avx2_2rounds : 
+   rela st1{1} st2{1} s{2} ==> rela res{1}.`1 res{1}.`2 res{2}.
+proof.
+  proc => /=.
+  call s_avx2_sum_states.
+  call s_avx2_chacha20_rounds.
+  by call s_avx2_copy_states;wp;skip.
+qed.
+
+
+(* ------------------------------------------------------------ *)
+
+equiv hacl_s_avx2_2rounds : 
+  Chacha20_hacl.M.hacl_2rounds ~
+  Chacha20_s_avx2.M.avx2_2rounds : 
+   rela st1{1} st2{1} s{2} ==> rela res{1}.`1 res{1}.`2 res{2}.
+proof.
+  transitivity Chacha20_hacl_x2.M.hacl_2rounds
+    (={st1,st2} ==> ={res}) 
+    (rela st1{1} st2{1} s{2} ==> rela res{1}.`1 res{1}.`2 res{2}) => //.
+  + by move=> &1 &2 h;exists (st1{1}, st2{1}).
+  + by apply hacl_x2_double.
+  by apply s_avx2_2rounds.
+qed.
+
